removal of self loops from MMA using syntactic properties of the generic compiler is much easier now than it was for MM !! Getting boundedness properties for jump addresses may require some more work though !

theories/MinskyMachines/MMA/mma_no_self.v
@@ -8,14 +8,15 @@
 (**************************************************************)
 
 (* * Minsky machines to FRACTRAN programs *)
-(* ** Removal of self-loops in MMAs *)
+(* ** Removal of self-loops in MMAs using syntactic and semantic
+      properties of the generic compiler *)
 
 Require Import List Arith Lia.
 
 Import ListNotations.
 
 From Undecidability.Shared.Libs.DLW
-  Require Import utils pos vec subcode sss compiler.
+  Require Import utils pos vec subcode sss compiler compiler_correction.
 
 From Undecidability.MinskyMachines.MMA
   Require Import mma_defs.
@@ -25,13 +26,11 @@ Set Implicit Arguments.
 Tactic Notation "rew" "length" := autorewrite with length_db.
 
 Local Notation "e #> x" := (vec_pos e x).
-Local Notation "e [ v / x ]" := (vec_change e x v).
+Local Notation "e [ v / x ]" := (vec_change e x v). (* clashes with ListNotations below *)
 
 Local Notation "I // s -1> t" := (mma_sss I s t).
-Local Notation "P // s -[ k ]-> t" := (sss_steps (@mma_sss _) P k s t).
 Local Notation "P // s -+> t" := (sss_progress (@mma_sss _) P s t).
 Local Notation "P // s ->> t" := (sss_compute (@mma_sss _) P s t).
-Local Notation "P // s '~~>' t" := (sss_output (@mma_sss _) P s t).
 Local Notation "P // s ↓" := (sss_terminates (@mma_sss _) P s). 
 
 Section no_self_loops.
@@ -75,7 +74,7 @@ Section remove_self_loops.
     Local Definition ic i ρ :=
       match ρ with
         | INCₐ x   => [ INCₐ x ]
-        | DECₐ x j => [ DECₐ x (2+lnk i) ;
+        | DECₐ x j => [ DECₐ x (3+lnk i) ;
                         INCₐ x ;
                         DECₐ x (5+lnk i) ;
                         INCₐ x ;
@@ -90,11 +89,45 @@ Section remove_self_loops.
 
   End instr_compiler.
 
+  Hint Resolve subcode_refl : core.
+
+  Local Fact ic_correct : instruction_compiler_sound ic (@mma_sss _) (@mma_sss _) eq.
+  Proof.
+    intros lnk I i1 v1 i2 v2 w1.
+    change i1 with (fst (i1,v1)) at 2 3 4 5 6 7.
+    change i2 with (fst (i2,v2)) at 2.
+    change v1 with (snd (i1,v1)) at 5.
+    change v2 with (snd (i2,v2)) at 3.
+    generalize (i1,v1) (i2,v2); intros st1 st2; clear i1 v1 i2 v2.
+    induction 1 as [ i x v | i x k v H | i x k v u H ]; simpl.
+    + intros -> <-. 
+      exists (vec_change v x (S (v#>x))); split; auto.
+      mma sss INC with x.
+      mma sss stop.
+    + intros -> <-.
+      exists v; split; auto.
+      mma sss DEC zero with x (S (S (S (lnk i)))).
+      mma sss INC with x.
+      mma sss DEC S with x (S (S (S (S (S (lnk i)))))) (v#>x); rew vec.
+      mma sss stop.
+    + intros _ <-.
+      exists (vec_change v x u); split; auto.
+      mma sss DEC S with x (S (S (S (lnk i)))) u.
+      mma sss INC with x.
+      1: do 2 apply subcode_cons; subcode_tac.
+      mma sss DEC S with x (lnk k) u; rew vec.
+      mma sss stop.
+  Qed.
+
   Section no_self_loops. 
 
     Let gc := generic_syntactic_compiler _ _ il_le il_ic_length.
 
-    Fact gc_no_self_loops P i : mma_no_self_loops (i,cs_code gc P i).
+    Variables (P : list (mm_instr (pos n))).
+
+    Let Q := cs_code gc (1,P) 1.
+
+    Local Fact gc_no_self_loops : mma_no_self_loops (1,Q).
     Proof.
       generalize (cs_not_between gc).
       destruct gc as [ lnk code H0 H1 H2 H3 H4 H5 H6 ]; simpl; clear gc; intro H7.
@@ -108,10 +141,48 @@ Section remove_self_loops.
         * inversion E2; lia.
         * easy.
         * inversion E2; clear E2.
-          specialize (H7 P i j' k).
-          apply H2 with (i := i) in G1; simpl in G1; lia.
+          specialize (H7 (1,P) 1 j' k).
+          apply H2 with (i := 1) in G1; simpl in G1; lia.
         * now apply subcode_nil_invert in G2.
       Qed.
+
+  (*
+
+    Local Fact gc_bounded j x k : (j,DECₐ x k::nil) <sc (i,Q) -> k < i+length Q.
+    Proof.
+      destruct gc as [ lnk code H0 H1 H2 H3 H4 H5 H6 ]; clear gc.
+      simpl in Q.
+      intros H.
+      apply H6 in H as (k' & [ x' | x' j' ] & G1 & G2); simpl ic in G2.
+      + apply subcode_cons_invert_right in G2 as [ (_ & ?) | G2 ]; try easy.
+        now apply subcode_nil_invert in G2.
+      + generalize G1; intros G0.
+        apply H5 with (i := i) in G0; fold Q in G0; apply subcode_length' in G0; simpl in G0.
+        apply subcode_in_code with (i := k') in G1.
+        2: simpl; lia.
+        apply H1 with (i := i) in G1; fold Q in G1; red in G1; unfold code_end, code_start in G1.
+        unfold fst, snd in G1.
+        admit.
+    Admitted.
+
+  *)
+
+    Hint Resolve il_ic_length ic_correct mma_sss_total_ni : core.
+
+    Let lnk := cs_link gc (1,P) 1.
+
+    Theorem mma_remove_self_loops : { Q | mma_no_self_loops (1,Q)
+                                       /\ forall v, (1,P) // (1,v) ↓ <-> (1,Q) // (1,v) ↓ }.
+    Proof.
+      exists Q; split.
+      + apply gc_no_self_loops.
+      + intros; apply compiler_syntactic_term_equiv with (simul := eq); auto.
+        * apply mma_sss_total_ni.
+        * apply mma_sss_fun.
+    Qed.
+
+    (* DLW to YF: on may want more information like a bound on jumps
+                  in the loop-free program *)
 
   End no_self_loops.
 
